AwsCryptographicMaterialProviders/dafny/AwsCryptographyKeyStoreAdmin/src/MutationStateStructures.dfy
@@ -48,9 +48,10 @@ module {:options "/functionSyntax:4" } MutationStateStructures {
     && (input.terminalKmsArn.Some? ==> KmsArn.ValidKmsArn?(input.terminalKmsArn.value))
     && (input.terminalEncryptionContext.Some? ==>
           && |input.terminalEncryptionContext.value| > 0
-          &&  forall k <- input.terminalEncryptionContext.value :: |k| > 0 && |input.terminalEncryptionContext.value[k]| > 0
-                                                                && |Structure.SelectCustomEncryptionContextAsString(input.terminalEncryptionContext.value)| == 0
-                                                                && input.terminalEncryptionContext.value.Keys !! Structure.BRANCH_KEY_RESTRICTED_FIELD_NAMES)
+          &&  forall k <- input.terminalEncryptionContext.value ::
+               && |k| > 0 && |input.terminalEncryptionContext.value[k]| > 0
+               && |Structure.SelectCustomEncryptionContextAsString(input.terminalEncryptionContext.value)| == 0
+               && input.terminalEncryptionContext.value.Keys !! Structure.BRANCH_KEY_RESTRICTED_FIELD_NAMES)
     && !(input.terminalKmsArn.None? && input.terminalEncryptionContext.None?)
   }
 
