AwsCryptographicMaterialProviders/dafny/AwsCryptographyKeyStoreAdmin/test/Mutations/TestInitMutActiveAndBeaconAreInSameState.dfy
@@ -1,0 +1,90 @@
+// Copyright Amazon.com Inc. or its affiliates. All Rights Reserved.
+// SPDX-License-Identifier: Apache-2.0
+
+include "../../src/Index.dfy"
+include "../../../AwsCryptographyKeyStore/test/CleanupItems.dfy"
+include "../../../AwsCryptographyKeyStore/test/Fixtures.dfy"
+include "../../../AwsCryptographyKeyStore/Model/AwsCryptographyKeyStoreTypes.dfy"
+include "../AdminFixtures.dfy"
+
+// Tests that if the Active & Beacon are in different states,
+// Initialize Mutations fails
+module {:options "/functionSyntax:4" } TestInitMutActiveAndBeaconAreInSameState {
+  import Types = AwsCryptographyKeyStoreAdminTypes
+  import KeyStoreAdmin
+  import KeyStore
+  import KeyStoreTypes = AwsCryptographyKeyStoreTypes
+  import opened Wrappers
+  import Fixtures
+  import AdminFixtures
+  import UUID
+  import CleanupItems
+  import KMS = Com.Amazonaws.Kms
+  import DDB = Com.Amazonaws.Dynamodb
+  import DefaultKeyStorageInterface
+  import Time
+  import Structure
+  import String = StandardLibrary.String
+  import UTF8
+  import opened StandardLibrary.UInt
+
+  const sadCaseId := "test-mutations-active-and-beacon-are-in-same-state"
+  const customEC := "aws-crypto-ec:Koda"
+  const kmsId: string := Fixtures.keyArn
+  const physicalName: string := Fixtures.branchKeyStoreName
+  const logicalName: string := Fixtures.logicalKeyStoreName
+  const testLogPrefix := "\nTestMutationsActiveAndBeaconAreInSameState :: TestSadCase :: "
+
+  method {:test} {:vcs_split_on_every_assert} TestSadCase()
+  {
+    print " running";
+
+    // expect false; // disable test till other investigation is done
+    var ddbClient :- expect DDB.DynamoDBClient();
+    var kmsClient :- expect KMS.KMSClient();
+
+    var underTest :- expect AdminFixtures.DefaultAdmin(ddbClient?:=Some(ddbClient));
+    var strategy :- expect AdminFixtures.DefaultKeyManagerStrategy(kmsClient?:=Some(kmsClient));
+    // Recommend commenting this out while developing this method,
+    // and just ignore the modifies exeptions,
+    // and then re-enabling it once everything is safe
+    // assume {:axiom} underTest.Modifies == {};
+
+    // var uuid :- expect UUID.GenerateUUID();
+    var testId := sadCaseId; // + "-" + uuid;
+
+    var kodaBytes :- expect UTF8.Encode("Koda");
+    var isADogBytes :- expect UTF8.Encode("is a dog.");
+    var originalEC := map[kodaBytes := isADogBytes];
+    AdminFixtures.CreateHappyCaseId(id:=testId, versionCount:=1, customEC:=originalEC);
+
+    print testLogPrefix + " Created the legit test items with 2 versions! testId: " + testId + "\n";
+
+    var _ :- expect AdminFixtures.AddAttributeWithoutLibrary(id := testId);
+
+    print testLogPrefix + " Violated the active and latest. testId: " + testId + "\n";
+
+    var timestamp :- expect Time.GetCurrentTimeStamp();
+    var newCustomEC: KeyStoreTypes.EncryptionContextString := map["Koda" := timestamp];
+    var mutationsRequest := Types.Mutations(terminalEncryptionContext := Some(newCustomEC));
+    var initInput := Types.InitializeMutationInput(
+      branchKeyIdentifier := testId,
+      mutations := mutationsRequest,
+      strategy := Some(strategy));
+    var initializeOutput? := underTest.InitializeMutation(initInput);
+
+    expect initializeOutput?.Failure?, "Initialize Mutation did not detect drifted Active & Beacon!";
+    match initializeOutput?.error {
+      case UnexpectedStateException(message) =>
+        expect true;
+      case _ => expect false, "Initialize Mutation should fail with Unexpected State Exception if Active & Beacon are different!";
+    }
+    print testLogPrefix + " Initialize Mutation met expectations\n";
+    print "TestInitMutActiveAndBeaconAreInSameState.TestSadCase: ";
+  }
+}
+// testId: test-mutate-encryption-add-value-da72ac87-5d28-4b84-8a56-96b4ea6e4326
+
+// TestEncryptionContextAddValue :: TestHappyCase ::  Violated the active and latest. testId: test-mutate-encryption-add-value-da72ac87-5d28-4b84-8a56-96b4ea6e4326
+
+        // dafny/AwsCryptographyKeyStoreAdmin/test/Mutations/TestEncryptionContextAddValue.dfy(89,28): Wrappers.Result.Failure(AwsCryptographyKeyStoreAdminTypes.Error.UnexpectedStateException(Beacon Item is not in the Original State! For Initialize Mutation to succeed, the ACTIVE & Beacon Key MUST be in the original state.))
